---
title: "Untitled"
format: html
editor: visual
---

$$
  \prod_i \prod_{j = 0}^{k - 2} \exp\left\{-[Y_i > j] e^{\eta_i + \gamma_j + \lambda}\right\}
    \times \left(1 - \exp\{-e^{\eta_i + \gamma_j + \lambda}\}\right)^{Y_i = j}
$$

$$
  \prod_i \prod_{j = 0}^{k - 2} \exp\left\{-[Y_i > j] e^{\eta_i + \gamma_j + \lambda}\right\}
    \times 
    \exp\left\{[Y_i = j](\eta_i + \gamma_j + \lambda) - Z_i e^{\eta_i + \gamma_j + \lambda}\right\}
$$

$$
  \prod_i \prod_{j = 0}^{k - 2}
    \exp\left\{[Y_i = j](\eta_i + \gamma_j + \lambda) - (Z_i [Y_i = j] e^{\eta_i + \gamma_j} + [Y_i > j] e^{\eta_i + \gamma_j}) e^\lambda\right\}
$$


$$
  \exp\left\{\lambda \sum_i [Y_i < k - 1] - e^\lambda e^{\eta_i}\left(Z_i [Y_i < k - 1] e^{\gamma_{Y_i}} + \sum_{j = 0}^{Y_i - 1} e^{\gamma_j}\right)\right\}
$$






